SLL_Prediction.v
@@ -8,548 +8,471 @@ Import ListNotations.
 Module SllPredictionFn (Import D : Defs.T).
 
   Module Export PC := PredictionCompleteFn D.
+  
+  (* First, some static analysis over a grammar *)
 
-  Module SLL.
+  Lemma suffix_frame_eq_dec :
+    forall fr fr' : suffix_frame, {fr = fr'} + {fr <> fr'}.
+  Proof.
+    repeat decide equality; try apply t_eq_dec; try apply nt_eq_dec.
+  Qed.
 
-    (* First, some static analysis over a grammar *)
-    Inductive pos : Type :=
-    | Pos : option nonterminal -> list symbol -> pos.
+  Module MDT_SF.
+    Definition t       := suffix_frame.
+    Definition eq_dec  := suffix_frame_eq_dec.
+  End MDT_SF.
+  Module SF_as_DT      := Make_UDT(MDT_SF).
+  Module FrameSet      := MSetWeakList.Make SF_as_DT.
+  Module FrameSetFacts := WFactsOn SF_as_DT FrameSet.
+  Module FrameMap      := FMapWeakList.Make SF_as_DT.
 
-    Definition sll_stack := (pos * list pos)%type.
+  Definition edge := (suffix_frame * suffix_frame)%type.
 
-    Lemma pos_eq_dec :
-      forall p p' : pos, {p = p'} + {p <> p'}.
-    Proof.
-      repeat decide equality; try apply t_eq_dec; try apply nt_eq_dec.
-    Qed.
+  Definition src (e : edge) : suffix_frame := fst e.
+  Definition dst (e : edge) : suffix_frame := snd e.
 
-    Module MDT_Pos.
-      Definition t := pos.
-      Definition eq_dec := pos_eq_dec.
-    End MDT_Pos.
-    Module Pos_as_DT   := Make_UDT(MDT_Pos).
-    Module Pset  := MSetWeakList.Make Pos_as_DT.
-    Module PsetF := WFactsOn Pos_as_DT Pset.
-    Module Pmap  := FMapWeakList.Make Pos_as_DT.
+  Lemma edge_eq_dec :
+    forall e e' : edge, {e = e'} + {e <> e'}.
+  Proof.
+    repeat decide equality; try apply t_eq_dec; try apply nt_eq_dec.
+  Qed.
 
-    Definition edge := (pos * pos)%type.
+  Module MDT_Edge.
+    Definition t      := edge.
+    Definition eq_dec := edge_eq_dec.
+  End MDT_Edge.
+  Module Edge_as_DT   := Make_UDT(MDT_Edge).
+  Module EdgeSet      := MSetWeakList.Make Edge_as_DT.
+  Module EdgeSetFacts := WFactsOn Edge_as_DT EdgeSet.
 
-    Definition src (e : edge) : pos := fst e.
+  Module FS := FrameSet.
+  Module FM := FrameMap.
+  Module ES := EdgeSet.
+  
+  Definition oneToMany {A B : Type} (s : A) (ds : list B) : list (A * B) :=
+    map (pair s) ds.
 
-    Definition dst (e : edge) : pos := snd e.
+  Definition beqNt x x' : bool :=
+    match nt_eq_dec x' x with
+    | left _ => true
+    | right _ => false
+    end.
 
-    Lemma edge_eq_dec :
-      forall e e' : edge, {e = e'} + {e <> e'}.
-    Proof.
-      repeat decide equality; try apply t_eq_dec; try apply nt_eq_dec.
-    Qed.
+  Fixpoint prodsOf (x : nonterminal) (ps : list production) := 
+    filter (fun p => beqNt x (lhs p)) ps.
 
-    Module MDT_Edge.
-      Definition t := edge.
-      Definition eq_dec := edge_eq_dec.
-    End MDT_Edge.
-    Module Edge_as_DT   := Make_UDT(MDT_Edge).
-    Module E  := MSetWeakList.Make Edge_as_DT.
-    Module EF := WFactsOn Edge_as_DT E.
+  Fixpoint pushEdges' (g : grammar) (x : nonterminal) (ys : list symbol) : list edge :=
+    match ys with 
+    | []          => []
+    | T _ :: ys'  => pushEdges' g x ys'
+    | NT y :: ys' =>
+      let es := map (fun rhs => (SF (Some x) ys, SF (Some y) rhs))
+                    (rhssForNt g y)
+      in  es ++ pushEdges' g x ys'
+    end.
 
-    Definition oneToMany {A B : Type} (s : A) (ds : list B) : list (A * B) :=
-      map (pair s) ds.
+  Definition pushEdges (g : grammar) : list edge :=
+    flat_map (fun p => pushEdges' g (lhs p) (rhs p)) g.
 
-    Definition beqNt x x' : bool :=
-      match nt_eq_dec x' x with
-      | left _ => true
-      | right _ => false
-      end.
+  Fixpoint returnEdges' (x : nonterminal) (ys : list symbol) : list edge :=
+    match ys with
+    | []          => []
+    | T _ :: ys'  => returnEdges' x ys'
+    | NT y :: ys' =>
+      (SF (Some y) [], SF (Some x) ys') :: returnEdges' x ys'
+    end.
 
-    Fixpoint prodsOf (x : nonterminal) (ps : list production) := 
-      filter (fun p => beqNt x (lhs p)) ps.
+  Definition returnEdges (g : grammar) : list edge :=
+    flat_map (fun p => returnEdges' (lhs p) (rhs p)) g.
 
-    Fixpoint pushEdges' (g : grammar) (x : nonterminal) (ys : list symbol) : list edge :=
-      match ys with 
-      | []          => []
-      | T _ :: ys'  => pushEdges' g x ys'
-      | NT y :: ys' =>
-        let es := map (fun rhs => (Pos (Some x) ys, Pos (Some y) rhs))
-                      (rhssForNt g y)
-        in  es ++ pushEdges' g x ys'
-      end.
+  Definition finalEdges g : list edge :=
+    map (fun x => (SF (Some x) [], SF None [])) (lhss g).
 
-    Definition pushEdges (g : grammar) : list edge :=
-      flat_map (fun p => pushEdges' g (lhs p) (rhs p)) g.
+  Definition fromEdgelist (es : list edge) : ES.t :=
+    fold_right ES.add ES.empty es.
 
-    Fixpoint returnEdges' (x : nonterminal) (ys : list symbol) : list edge :=
-      match ys with
-      | []          => []
-      | T _ :: ys'  => returnEdges' x ys'
-      | NT y :: ys' =>
-        (Pos (Some y) [], Pos (Some x) ys') :: returnEdges' x ys'
-      end.
+  Definition epsilonEdges g : list edge :=
+    pushEdges g ++ returnEdges g ++ finalEdges g.
 
-    Definition returnEdges (g : grammar) : list edge :=
-      flat_map (fun p => returnEdges' (lhs p) (rhs p)) g.
+  Fixpoint dsts (es : list edge) (s : suffix_frame) : list suffix_frame :=
+    match es with
+    | []             => []
+    | (s', d) :: es' =>
+      if suffix_frame_eq_dec s' s then d :: dsts es' s else dsts es' s
+    end.
 
-    Definition finalEdges g : list edge :=
-      map (fun x => (Pos (Some x) [], Pos None [])) (lhss g).
+  Definition mem (e : edge) (es : list edge) : bool :=
+    if in_dec edge_eq_dec e es then true else false.
 
-    Definition fromEdgelist (es : list edge) : E.t :=
-      fold_right E.add E.empty es.
+  Definition newEdges' (es : list edge) (e : edge) : list edge :=
+    let (a, b) := e in
+    let cs     := filter (fun c => negb (mem (a, c) es)) (dsts es b)
+    in  oneToMany a cs.
 
-    Definition epsilonEdges g : list edge :=
-      pushEdges g ++ returnEdges g ++ finalEdges g.
+  Definition newEdges (es : list edge) : list edge :=
+    flat_map (newEdges' es) es.
 
-    Fixpoint dsts (es : list edge) (s : pos) : list pos :=
-      match es with
-      | []             => []
-      | (s', d) :: es' =>
-        if pos_eq_dec s' s then d :: dsts es' s else dsts es' s
-      end.
+  Definition sources es := map src es.
+  Definition dests   es := map dst es.
 
-    Definition mem (e : edge) (es : list edge) : bool :=
-      if in_dec edge_eq_dec e es then true else false.
+  Definition allEdges es := 
+    let ss := sources es in
+    let ds := dests   es in
+    flat_map (fun s => oneToMany s ds) ss.
 
-    Definition newEdges' (es : list edge) (e : edge) : list edge :=
-      let (a, b) := e in
-      let cs     := filter (fun c => negb (mem (a, c) es)) (dsts es b)
-      in  oneToMany a cs.
+  Definition stable (fr : suffix_frame) : bool :=
+    match fr with
+    | SF None []             => true
+    | SF (Some x) (T _ :: _) => true
+    | _                      => false
+    end.
 
-    Definition newEdges (es : list edge) : list edge :=
-      flat_map (newEdges' es) es.
+  Fixpoint stablePositions' x ys : list suffix_frame :=
+    match ys with
+    | []          => []
+    | T a :: ys'  => SF (Some x) ys :: stablePositions' x ys'
+    | NT _ :: ys' => stablePositions' x ys'
+    end.
 
-    Definition sources es := map src es.
-    Definition dests   es := map dst es.
+  Definition stablePositions (g : grammar) : list suffix_frame :=
+    SF None [] :: flat_map (fun p => stablePositions' (lhs p) (rhs p)) g.
 
-    Definition allEdges es := 
-      let ss := sources es in
-      let ds := dests   es in
-      flat_map (fun s => oneToMany s ds) ss.
+  (* might not be necessary *)
+  Definition reflEdges (g : grammar) : list edge :=
+    map (fun p => (p, p)) (stablePositions g).
 
-    Definition stable (p : pos) : bool :=
-      match p with
-      | Pos None []             => true
-      | Pos (Some x) (T _ :: _) => true
-      | _                       => false
-      end.
+  Definition m (es : list edge) : nat :=
+    ES.cardinal (ES.diff (fromEdgelist (allEdges es)) (fromEdgelist es)).
 
-    Fixpoint stablePositions' x ys : list pos :=
-      match ys with
-      | []          => []
-      | T a :: ys'  => Pos (Some x) ys :: stablePositions' x ys'
-      | NT _ :: ys' => stablePositions' x ys'
-      end.
+  Axiom magic : forall A, A.
 
-    Definition stablePositions (g : grammar) : list pos :=
-      Pos None [] :: flat_map (fun p => stablePositions' (lhs p) (rhs p)) g.
+  Program Fixpoint transClosure (es : list edge)
+          { measure (m es) } : list edge :=
+    let es' := newEdges es in
+    match es' as es'' return es' = es'' -> _ with
+    | []     => fun _   => es
+    | _ :: _ => fun heq => transClosure (es' ++ es)
+    end eq_refl.
+  Next Obligation.
+    rewrite heq; simpl.
+    unfold m.
+    apply magic.
+  Defined.
 
-    Definition reflEdges (g : grammar) : list edge :=
-      map (fun p => (p, p)) (stablePositions g).
+  Definition dstStable (e : edge) : bool :=
+    let (_, b) := e in stable b.
 
-    Definition m (es : list edge) : nat :=
-      E.cardinal (E.diff (fromEdgelist (allEdges es)) (fromEdgelist es)).
+  Definition stableEdges (es : list edge) : list edge :=
+    filter dstStable es.
 
-    Axiom magic : forall A, A.
+  Definition mkGraphEdges (g : grammar) : list edge :=
+    stableEdges (transClosure (epsilonEdges g)) ++ (reflEdges g).
 
-    Program Fixpoint transClosure (es : list edge)
-            { measure (m es) } : list edge :=
-      let es' := newEdges es in
-      match es' as es'' return es' = es'' -> _ with
-      | []     => fun _   => es
-      | _ :: _ => fun heq => transClosure (es' ++ es)
-      end eq_refl.
-    Next Obligation.
-      rewrite heq; simpl.
-      unfold m.
-      apply magic.
-    Defined.
-
-    Definition destStable (e : edge) : bool :=
-      let (_, b) := e in stable b.
-
-    Definition stableEdges (es : list edge) : list edge :=
-      filter destStable es.
-
-    Definition mkGraphEdges (g : grammar) : list edge :=
-      stableEdges (transClosure (epsilonEdges g)) ++ (reflEdges g).
-
-    (* A closure graph is a map where each key K is a grammar position
+  (* A closure graph is a map where each key K is a grammar position
      and each value V is a set of positions that are epsilon-reachable from K *)
-    Definition closure_map := Pmap.t Pset.t.
+  Definition closure_map := FM.t FS.t.
 
-    Definition addEdge (e : edge) (m : closure_map) : closure_map :=
-      let (k, v) := e in
-      match Pmap.find k m with
-      | Some vs => Pmap.add k (Pset.add v vs) m
-      | None    => Pmap.add k (Pset.singleton v) m
-      end.
+  Definition addEdge (e : edge) (m : closure_map) : closure_map :=
+    let (k, v) := e in
+    match FM.find k m with
+    | Some vs => FM.add k (FS.add v vs) m
+    | None    => FM.add k (FS.singleton v) m
+    end.
 
-    Definition fromEdges (es : list edge) : closure_map :=
-      fold_right addEdge (Pmap.empty Pset.t) es.
+  Definition fromEdges (es : list edge) : closure_map :=
+    fold_right addEdge (FM.empty FS.t) es.
 
-    Definition mkGraph (g : grammar) : closure_map :=
-      fromEdges (mkGraphEdges g).
+  Definition mkGraph (g : grammar) : closure_map :=
+    fromEdges (mkGraphEdges g).
 
-    Definition callSites (p : pos) (cm : closure_map) : list sll_stack :=
-      match Pmap.find p cm with
-      | Some ps => map (fun p' => (p', [])) (Pset.elements ps)
-      | None    => []
-      end.
+  Definition callSites (cm : closure_map) (fr : suffix_frame) : list suffix_frame :=
+    match FM.find fr cm with
+    | Some s => FS.elements s
+    | None   => []
+    end.
 
-    (* Now for the parts that correspond to the LL prediction module *)
-    
-    Record subparser := Sp { prediction : list symbol
-                             ; stack      : sll_stack }.
+  (* Now for the parts that correspond to the LL prediction module *)
 
-    (* "move" operation *)
+  (* "SLL closure" operation *)
 
-    Inductive subparser_move_result :=
-    | SpMoveSucc   : subparser -> subparser_move_result
-    | SpMoveReject : subparser_move_result
-    | SpMoveError  : prediction_error -> subparser_move_result.
-
-    Definition moveSp (tok : token) (sp : subparser) : subparser_move_result :=
-      match sp with
-      | Sp pred stk =>
-        match stk with
-        | (Pos _ [], [])            => SpMoveReject
-        | (Pos _ [], _ :: _)        => SpMoveError SpInvalidState
-        | (Pos _ (NT _ :: _), _)    => SpMoveError SpInvalidState
-        | (Pos o (T a :: suf), frs) =>
-          match tok with
-          | (a', _) =>
-            if t_eq_dec a' a then
-              SpMoveSucc (Sp pred (Pos o suf, frs))
-            else
-              SpMoveReject
+  Definition sllClosureStep (g  : grammar)
+                           (cm : closure_map)
+                           (av : NtSet.t)
+                           (sp : subparser) : subparser_closure_step_result :=
+    match sp with
+    | Sp pred (fr, frs) =>
+      match fr with
+      | SF o [] =>
+        match frs with
+        | [] =>
+          (* SLL-specific part -- simulate a return to all call sites *)
+          match o with
+          | None   => CstepDone [sp] (* maybe this is an error? *)
+          | Some x =>
+            let sps' := map (fun fr' => Sp pred (fr', [])) (callSites cm fr)
+            in  CstepDone sps'
           end
+        | SF _ [] :: _                       => CstepError SpInvalidState
+        | SF _ (T _ :: _) :: _               => CstepError SpInvalidState
+        | SF o_cr (NT x :: suf_cr) :: frs_tl =>
+          let stk':= (SF o_cr suf_cr, frs_tl) 
+          in  CstepK (NtSet.add x av) [Sp pred stk'] 
         end
-      end.
+      | SF _ (T _ :: _)    => CstepDone [sp]
+      | SF _ (NT x :: suf) =>
+        if NtSet.mem x av then
+          let sps' := map (fun rhs => Sp pred 
+                                         (SF (Some x) rhs, fr :: frs))
+                          (rhssForNt g x)
+          in  CstepK (NtSet.remove x av) sps' 
+        else if NtSet.mem x (allNts g) then
+               CstepError (SpLeftRecursion x)
+             else
+               CstepK NtSet.empty [] 
+      end
+    end.
 
-    Definition move_result := sum prediction_error (list subparser).
-
-    Fixpoint aggrMoveResults (rs : list subparser_move_result) : move_result :=
-      match rs with
-      | []       => inr []
-      | r :: rs' =>
-        match (r, aggrMoveResults rs') with
-        | (SpMoveError e, _)       => inl e
-        | (_, inl e)               => inl e
-        | (SpMoveSucc sp, inr sps) => inr (sp :: sps)
-        | (SpMoveReject, inr sps)  => inr sps
-        end
-      end.
-
-    Definition move (tok : token) (sps : list subparser) : move_result :=
-      aggrMoveResults (map (moveSp tok) sps).
-
-    (* "closure" operation *)
-
-    Inductive subparser_closure_step_result :=
-    | SpClosureStepDone  : list subparser -> subparser_closure_step_result
-    | SpClosureStepK     : NtSet.t -> list subparser -> subparser_closure_step_result
-    | SpClosureStepError : prediction_error -> subparser_closure_step_result.
-
-    Definition spClosureStep (g : grammar) (cm : closure_map) (av : NtSet.t) (sp : subparser) : 
-      subparser_closure_step_result :=
-      match sp with
-      | Sp pred (fr, frs) =>
-        match fr with
-        | Pos o [] =>
-          match frs with
-          | []                 =>
-            (* SLL-specific part -- simulate a return to all call sites *)
-            match o with
-            | None   => SpClosureStepDone [sp]
-            | Some x =>
-              let sps' := map (Sp pred) (callSites fr cm)
-              in  SpClosureStepDone sps'
-            end
-          | Pos _ [] :: _         => SpClosureStepError SpInvalidState
-          | Pos _ (T _ :: _) :: _ => SpClosureStepError SpInvalidState
-          | Pos o_cr (NT x :: suf_cr) :: frs_tl =>
-            let stk':= (Pos o_cr suf_cr, frs_tl) 
-            in  SpClosureStepK (NtSet.add x av) [Sp pred stk'] 
-          end
-        | Pos _ (T _ :: _)    => SpClosureStepDone [sp]
-        | Pos _ (NT x :: suf) =>
-          if NtSet.mem x av then
-            let sps' := map (fun rhs => Sp pred 
-                                           (Pos (Some x) rhs, fr :: frs))
-                            (rhssForNt g x)
-            in  SpClosureStepK (NtSet.remove x av) sps' 
-          else if NtSet.mem x (allNts g) then
-                 SpClosureStepError (SpLeftRecursion x)
-               else
-                 SpClosureStepK NtSet.empty [] 
-        end
-      end.
-
-    Definition closure_result := sum prediction_error (list subparser).
-
-    (* consider refactoring to short-circuit in case of error *)
-    Fixpoint aggrClosureResults (crs : list closure_result) : closure_result :=
-      match crs with
-      | [] => inr []
-      | cr :: crs' =>
-        match (cr, aggrClosureResults crs') with
-        | (inl e, _)          => inl e
-        | (inr _, inl e)      => inl e
-        | (inr sps, inr sps') => inr (sps ++ sps')
-        end
-      end.
-
-    Definition suffixFrameOf (p : pos) :=
-      match p with
-      | Pos _ ys => SF ys
-      end.
-
-    Definition suffixStackOf (stk : sll_stack) :=
-      let (fr, frs) := stk
-      in  (suffixFrameOf fr, map suffixFrameOf frs).
-    
-    Definition meas (g : grammar) (av : NtSet.t) (sp : subparser) : nat * nat :=
-      match sp with
-      | Sp _ stk =>
-        let stk' := suffixStackOf stk in
-        let m := maxRhsLength g in
-        let e := NtSet.cardinal av               
-        in  (stackScore stk' (1 + m) e, stackHeight stk')
-      end.
-
-    (*
-  Lemma meas_lt_after_return :
-    forall g sp sp' av av' pred suf' x frs,
-      sp = Sp pred (SF [], SF (NT x :: suf') :: frs)
-      -> sp' = Sp pred (SF suf', frs)
-      -> av' = NtSet.add x av
-      -> lex_nat_pair (meas g av' sp') (meas g av sp).
-  Proof.
-    intros g sp sp' av av' pred suf' x frs ? ? ?; subst.
-    pose proof (stackScore_le_after_return' suf' x) as hle.
-    eapply le_lt_or_eq in hle; eauto.
-    destruct hle as [hlt | heq]; sis.
-    - apply pair_fst_lt; eauto.
-    - rewrite heq; apply pair_snd_lt; auto.
-  Defined.
-
-  Lemma meas_lt_after_push :
-    forall g sp sp' fr fr' av av' pred suf x rhs frs,
-      sp     = Sp pred (fr, frs)
-      -> sp' = Sp pred (fr', fr :: frs)
-      -> fr  = SF (NT x :: suf)
-      -> fr' = SF rhs
-      -> av' = NtSet.remove x av
-      -> NtSet.In x av
-      -> In (x, rhs) g
-      -> lex_nat_pair (meas g av' sp') (meas g av sp).
-  Proof.
-    intros g sp sp' fr fr' av av' pred suf x rhs frs ? ? ? ? ? hi hi'; subst.
-    apply pair_fst_lt.
-    eapply stackScore_lt_after_push; sis; eauto.
-  Defined.
-
-  Lemma spClosureStep_meas_lt :
+  Lemma CstepK_sll_equiv_ll :
     forall (g      : grammar)
+           (cm     : closure_map)
            (sp sp' : subparser)
            (sps'   : list subparser)
            (av av' : NtSet.t),
-      spClosureStep g av sp = SpClosureStepK av' sps'
-      -> In sp' sps'
-      -> lex_nat_pair (meas g av' sp') (meas g av sp).
+      sllClosureStep g cm av sp = CstepK av' sps'
+      -> spClosureStep g av sp = CstepK av' sps'.
   Proof.
-    intros g sp sp' sps' av av' hs hi. 
-    unfold spClosureStep in hs; dmeqs h; tc; inv hs; try solve [inv hi].
-    - apply in_singleton_eq in hi; subst.
-      eapply meas_lt_after_return; eauto.
-    - apply in_map_iff in hi.
-      destruct hi as [rhs [heq hi]]; subst.
-      eapply meas_lt_after_push; eauto.
-      + apply NtSet.mem_spec; auto.
-      + apply rhssForNt_in_iff; auto.
+    intros g cm sp sp' sps' av av' hs; unfold sllClosureStep in hs; dms; tc.
   Defined.
-     *)
-    Lemma acc_after_step :
-      forall g cm sp sp' sps' av av',
-        spClosureStep g cm av sp = SpClosureStepK av' sps'
-        -> In sp' sps'
-        -> Acc lex_nat_pair (meas g av sp)
-        -> Acc lex_nat_pair (meas g av' sp').
-    Proof.
-      intros g cm sp sp' sps' av av' heq hi ha.
-      eapply Acc_inv; eauto.
-      apply magic.
-    Defined.
 
-    Fixpoint spClosure (g  : grammar)
-             (cm : closure_map)
-             (av : NtSet.t)
-             (sp : subparser)
-             (a  : Acc lex_nat_pair (meas g av sp)) : closure_result :=
-      match spClosureStep g cm av sp as r return spClosureStep g cm av sp = r -> _ with
-      | SpClosureStepDone sps'  => fun _  => inr sps'
-      | SpClosureStepError e    => fun _  => inl e
-      | SpClosureStepK av' sps' => 
-        fun hs => 
-          let crs := dmap sps' (fun sp' hin =>
-                                  spClosure g cm av' sp'
-                                            (acc_after_step _ _ _ _ _ _ _ hs hin a))
-          in  aggrClosureResults crs
-      end eq_refl.
+  Lemma acc_after_sll_step :
+    forall g cm sp sp' sps' av av',
+      sllClosureStep g cm av sp = CstepK av' sps'
+      -> In sp' sps'
+      -> Acc lex_nat_pair (meas g av sp)
+      -> Acc lex_nat_pair (meas g av' sp').
+  Proof.
+    intros g cm sp sp' sps' av av' heq hi ha.
+    eapply Acc_inv; eauto.
+    eapply spClosureStep_meas_lt; eauto.
+    eapply CstepK_sll_equiv_ll; eauto.
+  Defined.
 
-    Definition closure (g : grammar) (cm : closure_map) (sps : list subparser) :
-      sum prediction_error (list subparser) :=
-      aggrClosureResults (map (fun sp => spClosure g cm (allNts g) sp (lex_nat_pair_wf _)) sps).
+  Definition closure_result := sum prediction_error (list subparser).
 
-    (* SLL prediction *)
+  Fixpoint sllSpClosure (g  : grammar)
+                        (cm : closure_map)
+                        (av : NtSet.t)
+                        (sp : subparser)
+                        (a  : Acc lex_nat_pair (meas g av sp))
+                        : closure_result :=
+    match sllClosureStep g cm av sp as r return sllClosureStep g cm av sp = r -> _ with
+    | CstepDone sps'  => fun _  => inr sps'
+    | CstepError e    => fun _  => inl e
+    | CstepK av' sps' => 
+      fun hs => 
+        let crs :=
+            dmap sps' (fun sp' hin =>
+                         sllSpClosure g cm av' sp'
+                                      (acc_after_sll_step _ _ _ _ _ _ _ hs hin a))
+        in  aggrClosureResults crs
+    end eq_refl.
 
-    Definition finalConfig (sp : subparser) : bool :=
-      match sp with
-      | Sp _ (Pos None [], []) => true
-      | _                      => false
-      end.
+  Definition sllClosure (g : grammar) (cm : closure_map) (sps : list subparser) :
+    sum prediction_error (list subparser) :=
+    aggrClosureResults (map (fun sp => sllSpClosure g cm (allNts g) sp (lex_nat_pair_wf _)) sps).
 
-    Definition allPredictionsEqual (sp : subparser) (sps : list subparser) : bool :=
-      allEqual _ beqGamma sp.(prediction) (map prediction sps).
+  (* SLL prediction *)
 
-    Definition handleFinalSubparsers (sps : list subparser) : prediction_result :=
-      match filter finalConfig sps with
-      | []         => PredReject
-      | sp :: sps' => 
-        if allPredictionsEqual sp sps' then
-          PredSucc sp.(prediction)
-        else
-          PredAmbig sp.(prediction)
-      end.
+  Definition cache_key := (list subparser * terminal)%type.
 
-    Definition cache_key := (list subparser * terminal)%type.
+  Lemma cache_key_eq_dec : 
+    forall k k' : cache_key,
+      {k = k'} + {k <> k'}.
+  Proof.
+    repeat decide equality; try apply t_eq_dec; try apply nt_eq_dec.
+  Defined.
 
-    Lemma cache_key_eq_dec : 
-      forall k k' : cache_key,
-        {k = k'} + {k <> k'}.
-    Proof.
-      repeat decide equality; try apply t_eq_dec; try apply nt_eq_dec.
-    Defined.
+  Module MDT_CacheKey.
+    Definition t := cache_key.
+    Definition eq_dec := cache_key_eq_dec.
+  End MDT_CacheKey.
+  Module CacheKey_as_DT := Make_UDT(MDT_CacheKey).
+  Module Cache := FMapWeakList.Make CacheKey_as_DT.
+  Module CacheFacts := WFacts_fun CacheKey_as_DT Cache.
 
-    Module MDT_CacheKey.
-      Definition t := cache_key.
-      Definition eq_dec := cache_key_eq_dec.
-    End MDT_CacheKey.
-    Module CacheKey_as_DT := Make_UDT(MDT_CacheKey).
-    Module Cache := FMapWeakList.Make CacheKey_as_DT.
-    Module CacheFacts := WFacts_fun CacheKey_as_DT Cache.
-
-    (* A cache is a finite map with (list subparser * terminal) keys 
+  (* A cache is a finite map with (list subparser * terminal) keys 
      and (list subparser) values *)
-    Definition cache : Type := Cache.t (list subparser).
+  Definition cache : Type := Cache.t (list subparser).
 
-    Definition empty_cache : cache := Cache.empty (list subparser).
+  Definition empty_cache : cache := Cache.empty (list subparser).
 
-    (* To do: maybe only PredSucc and PredAmbig should carry an updated cache *)
-    Fixpoint sllPredict' (g : grammar) (cm : closure_map) (sps : list subparser) (ts : list token) (c : cache) : prediction_result * cache :=
-      match sps with
-      | []         => (PredReject, c)
-      | sp :: sps' =>
-        if allPredictionsEqual sp sps' then
-          (PredSucc sp.(prediction), c)
-        else
-          match ts with
-          | []            => (handleFinalSubparsers sps, c)
-          | (a, l) :: ts' =>
-            match Cache.find (sps, a) c with 
-            | Some sps' => sllPredict' g cm sps' ts' c
-            | None      => 
-              match move (a, l) sps with
+  (* To do: maybe only PredSucc and PredAmbig should carry an updated cache *)
+  Fixpoint sllPredict' (g : grammar) (cm : closure_map) (sps : list subparser) (ts : list token) (c : cache) : prediction_result * cache :=
+    match sps with 
+    | []         => (PredReject, c)
+    | sp :: sps' =>
+      if allPredictionsEqual sp sps' then
+        (PredSucc sp.(prediction), c)
+      else
+        match ts with
+        | []            => (handleFinalSubparsers sps, c)
+        | (a, l) :: ts' =>
+          match Cache.find (sps, a) c with 
+          | Some sps' => sllPredict' g cm sps' ts' c
+          | None      => 
+            match move (a, l) sps with
+            | inl msg => (PredError msg, c)
+            | inr mv  =>
+              match sllClosure g cm mv with
               | inl msg => (PredError msg, c)
-              | inr mv  =>
-                match closure g cm mv with
-                | inl msg => (PredError msg, c)
-                | inr cl  =>
-                  let c' := Cache.add (sps, a) cl c
-                  in  sllPredict' g cm cl ts' c'
-                end
+              | inr cl  =>
+                let c' := Cache.add (sps, a) cl c
+                in  sllPredict' g cm cl ts' c'
               end
             end
           end
-      end.
+        end
+    end.
 
-    Definition initSps (g : grammar) (x : nonterminal) : list subparser :=
-      map (fun rhs => Sp rhs (Pos (Some x) rhs, []))
-          (rhssForNt g x).
+  Definition sllInitSps (g : grammar) (x : nonterminal) : list subparser :=
+    map (fun rhs => Sp rhs (SF (Some x) rhs, []))
+        (rhssForNt g x).
 
-    Definition startState (g : grammar) (cm : closure_map)
-               (x : nonterminal) : sum prediction_error (list subparser) :=
-      closure g cm (initSps g x).
+  Definition startState (g : grammar) (cm : closure_map)
+             (x : nonterminal) : sum prediction_error (list subparser) :=
+    sllClosure g cm (sllInitSps g x).
 
-    Definition sllPredict (g : grammar) (cm : closure_map) (x : nonterminal)
-               (ts : list token) (c : cache) : prediction_result * cache :=
-      match startState g cm x with
-      | inl msg => (PredError msg, c)
-      | inr sps => sllPredict' g cm sps ts c
-      end.
+  Definition sllPredict (g : grammar) (cm : closure_map) (x : nonterminal)
+             (ts : list token) (c : cache) : prediction_result * cache :=
+    match startState g cm x with
+    | inl msg => (PredError msg, c)
+    | inr sps => sllPredict' g cm sps ts c
+    end.
 
-  Definition adaptivePredict g cm x stk ts c : prediction_result * SLL.cache :=
+  Definition adaptivePredict g cm x stk ts c : prediction_result * cache :=
     let sll_res := sllPredict g cm x ts c in
     match sll_res with
     | (PredAmbig _, _) => (llPredict g x stk ts, c)
     | _ => sll_res
     end.
 
-  End SLL.
-
   (* Equivalence of LL and SLL *)
-
+  
   Lemma sll'_ll'_equiv_succ :
     forall g cm sps sps' ts c c' ys,
-      SLL.sllPredict' g cm sps ts c = (PredSucc ys, c')
+      sllPredict' g cm sps ts c = (PredSucc ys, c')
       -> llPredict' g sps' ts = PredReject
          \/llPredict' g sps' ts = PredSucc ys.
   Proof.
     intros g cm sps sps' ts c c' ys hs.
-    unfold SLL.sllPredict' in hs.
+    unfold sllPredict' in hs.
     induction ts as [| t ts IH].
     - destruct sps as [| sp sps]; tc.
-      destruct (SLL.allPredictionsEqual sp sps) eqn:ha.
+      destruct (allPredictionsEqual sp sps) eqn:ha.
       + (* SLL all equal *)
+        inv hs.
         destruct sps' as [| sp' sps']; auto.
-        right.
+        right. simpl.
+        (* an invariant relating the LL and SLL subaparsers
+           should prove that SLL all equal -> LL all equal *)
   Abort.
-  
-  Lemma sll_ll_equiv_succ :
-    forall g cm fr frs x suf ts c c' ys,
-      no_left_recursion g
-      -> suffix_stack_wf g (fr, frs)
-      -> fr = SF (NT x :: suf)
-      -> SLL.sllPredict g cm x ts c = (PredSucc ys, c')
-      -> llPredict g x (fr, frs) ts = PredSucc ys.
-  Proof.
-    intros g cm fr frs x suf ts c c' ys hn hw ? hs; subst.
-    unfold SLL.sllPredict in hs.
-    destruct (SLL.startState g cm x) as [e | sps] eqn:hss; tc.
-    unfold llPredict.
-    destruct (startState g x _) as [e | sps'] eqn:hss'.
-    - (* lemma *)
-      destruct e as [ | x'].
-      + exfalso; eapply startState_never_returns_SpInvalidState; eauto.
-      + exfalso; eapply closure_never_finds_left_recursion; eauto.
-    - (* what do we know at this point?
+
+  (*
+Lemma sll_ll_equiv_succ :
+  forall g cm fr frs x suf ts c c' ys,
+    no_left_recursion g
+    -> suffix_stack_wf g (fr, frs)
+    -> fr = SF (NT x :: suf)
+    -> SLL.sllPredict g cm x ts c = (PredSucc ys, c')
+    -> llPredict g x (fr, frs) ts = PredSucc ys.
+Proof.
+  intros g cm fr frs x suf ts c c' ys hn hw ? hs; subst.
+  unfold SLL.sllPredict in hs.
+  destruct (SLL.startState g cm x) as [e | sps] eqn:hss; tc.
+  unfold llPredict.
+  destruct (startState g x _) as [e | sps'] eqn:hss'.
+  - (* lemma *)
+    destruct e as [ | x'].
+    + exfalso; eapply startState_never_returns_SpInvalidState; eauto.
+    + exfalso; eapply closure_never_finds_left_recursion; eauto.
+  - (* what do we know at this point?
          - sllPredict' succeeded, so there must be an sp in sps with label ys
          - there must also be an sp' in sps' with label ys *)
-     admit.
-  Abort.
+    admit.
+Abort.
 
-  Lemma adaptivePredict_equiv_llPredict :
-    forall g cm x stk ts c c' r,
-      SLL.adaptivePredict g cm x stk ts c = (r, c')
-      -> llPredict g x stk ts = r.
-  Proof.
-    intros g cm x stk ts c c' r ha.
-    unfold SLL.adaptivePredict in ha.
-    destruct (SLL.sllPredict _ _ _ _ _) as (r', c'') eqn:hs.
-    destruct r' as [ys | ys | | e]; inv ha; auto.
-    - (* PredSucc *)
-      admit.
-    - admit.
-    - admit.
-  Admitted.
-      
-  
-
+Lemma adaptivePredict_equiv_llPredict :
+  forall g cm x stk ts c c' r,
+    SLL.adaptivePredict g cm x stk ts c = (r, c')
+    -> llPredict g x stk ts = r.
+Proof.
+  intros g cm x stk ts c c' r ha.
+  unfold SLL.adaptivePredict in ha.
+  destruct (SLL.sllPredict _ _ _ _ _) as (r', c'') eqn:hs.
+  destruct r' as [ys | ys | | e]; inv ha; auto.
+  - (* PredSucc *)
+    admit.
+  - admit.
+  - admit.
+Admitted.
+*)
 End SllPredictionFn.
+
+(* Equivalence of LL and SLL *)
+(*
+Lemma sll'_ll'_equiv_succ :
+  forall g cm sps sps' ts c c' ys,
+    
+sllPredict' g cm sps ts c = (PredSucc ys, c')
+    -> llPredict' g sps' ts = PredReject
+       \/llPredict' g sps' ts = PredSucc ys.
+Proof.
+  intros g cm sps sps' ts c c' ys hs.
+  unfold SLL.sllPredict' in hs.
+  induction ts as [| t ts IH].
+  - destruct sps as [| sp sps]; tc.
+    destruct (SLL.allPredictionsEqual sp sps) eqn:ha.
+    + (* SLL all equal *)
+      destruct sps' as [| sp' sps']; auto.
+      right.
+Abort.
+
+Lemma sll_ll_equiv_succ :
+  forall g cm fr frs x suf ts c c' ys,
+    no_left_recursion g
+    -> suffix_stack_wf g (fr, frs)
+    -> fr = SF (NT x :: suf)
+    -> SLL.sllPredict g cm x ts c = (PredSucc ys, c')
+    -> llPredict g x (fr, frs) ts = PredSucc ys.
+Proof.
+  intros g cm fr frs x suf ts c c' ys hn hw ? hs; subst.
+  unfold SLL.sllPredict in hs.
+  destruct (SLL.startState g cm x) as [e | sps] eqn:hss; tc.
+  unfold llPredict.
+  destruct (startState g x _) as [e | sps'] eqn:hss'.
+  - (* lemma *)
+    destruct e as [ | x'].
+    + exfalso; eapply startState_never_returns_SpInvalidState; eauto.
+    + exfalso; eapply closure_never_finds_left_recursion; eauto.
+  - (* what do we know at this point?
+         - sllPredict' succeeded, so there must be an sp in sps with label ys
+         - there must also be an sp' in sps' with label ys *)
+    admit.
+Abort.
+
+Lemma adaptivePredict_equiv_llPredict :
+  forall g cm x stk ts c c' r,
+    SLL.adaptivePredict g cm x stk ts c = (r, c')
+    -> llPredict g x stk ts = r.
+Proof.
+  intros g cm x stk ts c c' r ha.
+  unfold SLL.adaptivePredict in ha.
+  destruct (SLL.sllPredict _ _ _ _ _) as (r', c'') eqn:hs.
+  destruct r' as [ys | ys | | e]; inv ha; auto.
+  - (* PredSucc *)
+    admit.
+  - admit.
+  - admit.
+Admitted.
+
+*)  
